src/FrameStack/Frames.v
@@ -1,4 +1,4 @@
-Require Export ScopingLemmas.
+Require Export ScopingLemmas Maps.
 
 Import ListNotations.
 
@@ -16,347 +16,127 @@ Inductive Frame : Set :=
 | FCons2 (v2 : Exp) (* [□ | v2] *).
 *)
 
+(* It is an inductive to have the "FParams" name *)
+(* This frame is used to handle parameter lists in a unified way to avoid
+  duplication *)
+Inductive ParamFrame : Set :=
+| FParams : list Val -> list Exp -> ParamFrame. (* v₁, v₂, ... vᵢ₋₁, □, eᵢ₊₁, ..., eₙ *)
+
 Inductive Frame : Set :=
-
-| FValues (lv : list ValueExpression) (le : list Expression)
-(* EValues (v, ..., v, _, e, ..., e) *)
-
-| FCons1 (hd : Expression)
-(* ECons hd _ *) (* Here the evaluation starts from the second expression. *)
-
-| FCons2 (tl : ValueExpression)
-(* ECons _ tl *)
-
-| FTuple (lv : list ValueExpression) (le : list Expression)
-(* ETuple (v, ..., v, _, e, ..., e) *)
-
-| FMap1 (lv : list (ValueExpression * ValueExpression))
-          (sn : Expression)
-          (le : list (Expression * Expression))
-(* EMap ((v,v), ..., (v,v), (_,sn), (e,e), ..., (e,e)) *)
-
-| FMap2 (lv : list (ValueExpression * ValueExpression))
-          (fs : ValueExpression)
-          (le : list (Expression * Expression))
-(* EMap ((v,v), ..., (v,v), (fs,_), (e,e), ..., (e,e)) *)
-
-| FCall   (f : string) (lv : list ValueExpression) (le : list Expression)
-(* ECall f (v, ..., v, _, e, ..., e) *)
-
-| FPrimOp (f : string) (lv : list ValueExpression) (le : list Expression)
-(* FPrimOp f (v, ..., v, _, e, ..., e) *)
-
-| FApp1 (l : list Expression)
-(* EApp _ (e, ..., e) *)
-
-| FApp2 (v : ValueExpression) (lv : list ValueExpression) (le : list Expression)
-(* EApp v (v, ..., v, _, e, ..., e) *)
-
-| FCase1 (l : list ((list Pattern) * Expression * Expression))
-(* ECase _ ((pl, e, e) ..., (lp, e, e)) *)
-
-(*| FCase2_p (v : ValueExpression)
-           (lp : list Pattern)
-           (ex : Expression)
-           (le : list ((list Pattern) * Expression * Expression)) *)
-| FCase2   (lv : list ValueExpression)
-           (lp : list Pattern)
-           (ex : Expression)
-           (le : list ((list Pattern) * Expression * Expression))
-           (lvp : list ValueExpression) (* the result of the pattern matching, only needed in the reduction rules *)
+| FValues (l : ParamFrame)
+| FCons1 (hd : Exp) (* [e1 | □] *)
+| FCons2 (tl : Val) (* [□ | v2] *)
+| FTuple (l : ParamFrame)
+| FMap (l : ParamFrame) (* maps are tricky: the list of pairs is flattened with `flatten_list`, which can be reversed by `deflatten_list` *)
+| FCall   (f : string) (l : ParamFrame)
+| FPrimOp (f : string) (l : ParamFrame)
+| FApp1 (l : list Exp)
+| FApp2 (v : Val) (l : ParamFrame)
+| FCase1 (l : list ((list Pat) * Exp * Exp))
+| FCase2   (lv : list Val)
+           (lp : list Pat)
+           (ex : Exp)
+           (le : list ((list Pat) * Exp * Exp))
+           (lvp : list Val)
+           (* the result of the pattern matching, only needed in the reduction rules *)
 (* ECase v ((lp, _, ex), ..., (lp, e, e)) *)
-(* FCase2_p means that the pattern matching was not done yet so the current guard expression (referenced by "_" or called the hole) does not need to be evaluated yet. *)
-(* FCase2_g means that the last pattern matched so the current guard needs to be evaluated, so tha guard expression does not need to be evaluated yet. *)
+(* FCase2_p means that the pattern matching was not done yet so the current guard Exp (referenced by "_" or called the hole) does not need to be evaluated yet. *)
+(* FCase2_g means that the last pattern matched so the current guard needs to be evaluated, so tha guard Exp does not need to be evaluated yet. *)
 
-
-| FLet   (l : nat) (e : Expression)
-(* ELet l _ e *)
-
-| FSeq   (e : Expression)
-(* ESeq _ e *)
-
-| FTry (vl1 : nat) (e2 : Expression) (vl2 : nat) (e3 : Expression)
-(* ETry _ vl1 e2 vl2 e3 *)
-
+| FLet   (l : nat) (e : Exp) (* let <x₁, ..., xₙ> = □ in e *)
+| FSeq   (e : Exp)           (* do □ e *)
+| FTry (vl1 : nat) (e2 : Exp) (vl2 : nat) (e3 : Exp)
+  (* try □ of <x₁, ..., xₙ> -> e₂ catch <xₙ₊₁, ..., xₙ₊ₘ> -> e₃ *)
 .
 
-(* Not needed*)
-(*
-Inductive frame_wf : Frame -> Prop :=
-| wf_app1 l : frame_wf (FApp1 l)
-| wf_app2 vl b l1 l2 :  Forall (fun v => VALCLOSED v) l2 -> frame_wf (FApp2 (EFun vl b) l1 l2)
-| wf_let v e : frame_wf (FLet v e)
-| wf_plus1 e : frame_wf (FPlus1 e)
-| wf_plus2 v : VALCLOSED v -> frame_wf (FPlus2 v)
-| wf_if p e2 e3 : frame_wf (FCase p e2 e3)
-| wf_cons1 e : frame_wf (FCons1 e)
-| wf_cons2 v : VALCLOSED v -> frame_wf (FCons2 v).
-*)
-
-(* Fill the hole in the frame *)
-(*Definition plug_f (F : Frame) (e : Exp) : Exp :=
+Definition closed_ParamFrame (F : ParamFrame) : Prop :=
 match F with
- | FApp1 l => EApp e l
- | FApp2 v l1 l2 => EApp v (l2 ++ [e] ++ l1)
- | FLet v e2 => ELet v e e2
- | FPlus1 e2 => EPlus e e2
- | FPlus2 v => EPlus v e
- | FCase p e2 e3 => ECase e p e2 e3
- | FCons1 e1 => ECons e1 e
- | FCons2 v2 => ECons e v2
-end.*)
+| FParams vl el => Forall (fun v => VALCLOSED v) vl /\
+                   Forall (fun e => EXPCLOSED e) el
+end.
 
-
-Definition plug_f (F : Frame) (e : Expression) : Expression :=
+Definition lengthParamFrame (F : ParamFrame) : nat :=
 match F with
- | FValues lv le   => Exp (EValues ((map Val lv) ++ (cons e nil) ++ le))
- | FCons1 hd       => Exp (ECons hd e)
- | FCons2 tl       => Exp (ECons e (Val tl))
- | FTuple lv le    => Exp (ETuple ((map Val lv) ++ (cons e nil) ++ le))
- 
- | FMap1 lv sn le  => 
-        Exp (EMap ((map (fun '(v1,v2) => (Val v1, Val v2)) lv) ++ (cons (e,sn) nil) ++ le))
- | FMap2 lv fs le  => 
-        Exp (EMap ((map (fun '(v1,v2) => (Val v1, Val v2)) lv) ++ (cons (Val fs, e) nil) ++ le))
- 
- | FCall f lv le   => Exp (ECall f ((map Val lv) ++ (cons e nil) ++ le))
- | FPrimOp f lv le => Exp (EPrimOp f ((map Val lv) ++ (cons e nil) ++ le))
- | FApp1 l         => Exp (EApp e l)
- | FApp2 v lv le   => Exp (EApp (Val v) ((map Val lv) ++ (cons e nil) ++ le))
- | FCase1 l        => Exp (ECase e l)
- | FCase2 lv lp ex le lvp => (*TODO: if vl is a list how do we plug it into an expression*)
-        Exp (ECase (Exp (EValues (map Val lv))) ((cons (lp,e,ex) nil) ++ le))
+| FParams vl el => S (length vl + length el) (* there is a box in the list! *)
+end.
+
+Inductive FCLOSED : Frame -> Prop :=
+| wf_values l : closed_ParamFrame l -> FCLOSED (FValues l)
+| wf_cons1 e : EXPCLOSED e -> FCLOSED (FCons1 e)
+| wf_cons2 v : VALCLOSED v -> FCLOSED (FCons2 v)
+| wf_tuple l : closed_ParamFrame l -> FCLOSED (FTuple l)
+| wf_map l : 
+  (exists n, lengthParamFrame l = 2 * n) ->
+  closed_ParamFrame l
+->
+  FCLOSED (FMap l)
+| wf_call f l : closed_ParamFrame l -> FCLOSED (FCall f l)
+| wf_primop f l : closed_ParamFrame l -> FCLOSED (FPrimOp f l)
+| wf_app1 l : Forall (fun e => EXPCLOSED e) l -> FCLOSED (FApp1 l)
+| wf_app2 v l : VALCLOSED v -> closed_ParamFrame l -> FCLOSED (FApp2 v l)
+| wf_case1 l : 
+  (forall i : nat,
+  i < Datatypes.length l ->
+  EXP PatListScope (nth i (map (fst >>> fst) l) [])
+  ⊢ nth i (map (fst >>> snd) l) (` VNil)) ->
+  (forall i : nat,
+        i < Datatypes.length l ->
+        EXP PatListScope (nth i (map (fst >>> fst) l) [])
+        ⊢ nth i (map snd l) (` VNil))
+->  
+  FCLOSED (FCase1 l)
+| wf_case2 vl pl e rest lvp :
+  Forall (fun v => VALCLOSED v) vl ->
+  Forall (fun v => VALCLOSED v) lvp (* Necessary if the frame is used out of context *) ->
+  VAL PatListScope pl ⊢ e ->
+  (forall i : nat,
+  i < Datatypes.length rest ->
+  EXP PatListScope (nth i (map (fst >>> fst) rest) [])
+  ⊢ nth i (map (fst >>> snd) rest) (` VNil)) ->
+  (forall i : nat,
+        i < Datatypes.length rest ->
+        EXP PatListScope (nth i (map (fst >>> fst) rest) [])
+        ⊢ nth i (map snd rest) (` VNil))
+->
+  FCLOSED (FCase2 vl pl e rest lvp)
+| wf_let vars e : EXP vars ⊢ e -> FCLOSED (FLet vars e)
+| wf_seq e : EXPCLOSED e -> FCLOSED (FSeq e)
+| wf_try vars1 vars2 e2 e3 :
+  EXP vars1 ⊢ e2 -> EXP vars2 ⊢ e3
+->
+  FCLOSED (FTry vars1 e2 vars2 e3)
+.
+
+Definition plug_params (F : ParamFrame) (e : Exp) : list Exp :=
+match F with
+| FParams vl el => map VVal vl ++ [e] ++ el
+end.
+
+Definition plug_f (F : Frame) (e : Exp) : Exp :=
+match F with
+ | FValues l   => °(EValues (plug_params l e))
+ | FCons1 hd   => °(ECons hd e)
+ | FCons2 tl   => °(ECons e (`tl))
+ | FTuple l    => °(ETuple (plug_params l e))
+ | FMap l      => °(EMap (deflatten_list (plug_params l e)))
+ | FCall f l   => °(ECall f (plug_params l e))
+ | FPrimOp f l => °(EPrimOp f (plug_params l e))
+ | FApp1 l     => °(EApp e l)
+ | FApp2 v l   => °(EApp (`v) (plug_params l e))
+ | FCase1 l    => °(ECase e l)
+ | FCase2 lv lp ex le lvp =>
+   °(ECase (°EValues (map VVal lv)) ([(lp,e,ex)] ++ le))
  (*| FCase2 v lp ex le lv => (* lv only carries information needed in the evaluation of ex *)
         Exp (ECase (Val v) ((cons (lp,e,ex) nil) ++ le))*)
  (*| FCase2_g v lp ex le =>
         Exp (ECase (Val v) ((cons (lp,e,ex) nil) ++ le)) *)
 
- | FLet l ex            => Exp (ELet l e ex)
- | FSeq ex              => Exp (ESeq e ex)
- | FTry vl1 e2 vl2 e3   => Exp (ETry e vl1 e2 vl2 e3)
+ | FLet l ex            => °(ELet l e ex)
+ | FSeq ex              => °(ESeq e ex)
+ | FTry vl1 e2 vl2 e3   => °(ETry e vl1 e2 vl2 e3)
 end.
 
 Definition FrameStack := list Frame.
 
-(* All Exp Closed *)
-(*Inductive FCLOSED : Frame -> Prop :=
-| fclosed_app1 l:
-  Forall (fun e => EXPCLOSED e) l
-->
-  FCLOSED (FApp1 l)
-| fclosed_app2 v l1 l2:
-  VALCLOSED v -> Forall (fun e => EXPCLOSED e) l1 -> Forall (fun e => VALCLOSED e) l2
-->
-  FCLOSED (FApp2 v l1 l2)
-| fclosed_let e2 v :
-  EXP 1 ⊢ e2
-->
-  FCLOSED (FLet v e2)
-| fclosed_plus1 e2:
-  EXPCLOSED e2
-->
-  FCLOSED (FPlus1 e2)
-| fclosed_plus2 v1:
-  VALCLOSED v1
-->
-  FCLOSED (FPlus2 v1)
-| fclosed_if e2 e3 p:
-  EXP pat_vars p ⊢ e2 -> EXPCLOSED e3
-->
-  FCLOSED (FCase p e2 e3)
-| fclosed_cons1 e1:
-  EXPCLOSED e1
-->
-  FCLOSED (FCons1 e1)
-| fclosed_cons2 v:
-  VALCLOSED v
-->
-  FCLOSED (FCons2 v). *)
-
-Inductive FCLOSED : Frame -> Prop :=
-| FCLOSED_FValues lv le :
-  (forall i, i < length lv -> VALCLOSED (nth i lv (VNil))) ->
-  (forall i, i < length le -> EXPCLOSED (nth i le (Val VNil)))
-  ->
-  FCLOSED (FValues lv le)
-
-| FCLOSED_FCons1 hd :
-  EXPCLOSED hd
-  ->
-  FCLOSED (FCons1 hd)
-
-| FCLOSED_FCons2 tl :
-  VALCLOSED tl
-  ->
-  FCLOSED (FCons2 tl)
-
-| FCLOSED_FTuple lv le :
-  (forall i, i < length lv -> VALCLOSED (nth i lv (VNil))) ->
-  (forall i, i < length le -> EXPCLOSED (nth i le (Val VNil)))
-  ->
-  FCLOSED (FTuple lv le)
-
-| FCLOSED_FMap1 lv sn le :
-  (forall i, i < length lv -> VALCLOSED (nth i (map fst lv) (VNil))) ->
-  (forall i, i < length lv -> VALCLOSED (nth i (map snd lv) (VNil))) ->
-  (forall i, i < length le -> EXPCLOSED (nth i (map fst le) (Val VNil))) ->
-  (forall i, i < length le -> EXPCLOSED (nth i (map snd le) (Val VNil))) ->
-  EXPCLOSED sn
-  ->
-  FCLOSED (FMap1 lv sn le)
-
-| FCLOSED_FMap2 lv fs le :
-  (forall i, i < length lv -> VALCLOSED (nth i (map fst lv) (VNil))) ->
-  (forall i, i < length lv -> VALCLOSED (nth i (map snd lv) (VNil))) ->
-  (forall i, i < length le -> EXPCLOSED (nth i (map fst le) (Val VNil))) ->
-  (forall i, i < length le -> EXPCLOSED (nth i (map snd le) (Val VNil))) ->
-  VALCLOSED fs
-  ->
-  FCLOSED (FMap2 lv fs le)
-
-| FCLOSED_FCall f lv le :
-  (forall i, i < length lv -> VALCLOSED (nth i lv (VNil))) ->
-  (forall i, i < length le -> EXPCLOSED (nth i le (Val VNil)))
-  ->
-  FCLOSED (FCall f lv le)
-
-| FCLOSED_FPrimOp f lv le :
-  (forall i, i < length lv -> VALCLOSED (nth i lv (VNil))) ->
-  (forall i, i < length le -> EXPCLOSED (nth i le (Val VNil)))
-  ->
-  FCLOSED (FPrimOp f lv le)
-
-| FCLOSED_FApp1 l :
-  (forall i, i < length l -> EXPCLOSED (nth i l (Val VNil)))
-  ->
-  FCLOSED (FApp1 l)
-
-| FCLOSED_FApp2 v lv le :
-  (forall i, i < length lv -> VALCLOSED (nth i lv (VNil))) ->
-  (forall i, i < length le -> EXPCLOSED (nth i le (Val VNil))) ->
-  VALCLOSED v
-  ->
-  FCLOSED (FApp2 v lv le)
-
-| FCLOSED_FCase1 l :
-  (forall i, i < length l -> EXP (patternListScope (nth i (map fst (map fst l)) nil)) ⊢ (nth i (map snd (map fst l)) (Val VNil))) ->
-  (forall i, i < length l -> EXP (patternListScope (nth i (map fst (map fst l)) nil)) ⊢ (nth i (map snd l) (Val VNil)))
-  ->
-  FCLOSED (FCase1 l)
-  
-  
-| FCLOSED_FCase2 lv lp ex le lvp :
-  (forall i, i < length le -> EXP (patternListScope (nth i (map fst (map fst le)) nil)) ⊢ (nth i (map snd (map fst le)) (Val VNil))) ->
-  (forall i, i < length le -> EXP (patternListScope (nth i (map fst (map fst le)) nil)) ⊢ (nth i (map snd le) (Val VNil))) ->
-  (forall i, i < length lv -> VALCLOSED (nth i lv (VNil))) ->
-  (forall i, i < length lvp -> VALCLOSED (nth i lvp (VNil))) -> (*TODO it will stay for now, but not sure if needed *)
-  EXP (patternListScope lp) ⊢ ex
-  ->
-  FCLOSED (FCase2 lv lp ex le lvp)
-(*
-| FCLOSED_FCase2 v lp ex le lv:
-  (forall i, i < length le -> EXP (patternListScope (nth i (map fst (map fst le)) nil)) ⊢ (nth i (map snd (map fst le)) (Val VNil))) ->
-  (forall i, i < length le -> EXP (patternListScope (nth i (map fst (map fst le)) nil)) ⊢ (nth i (map snd le) (Val VNil))) ->
-  (forall i, i < length lv -> VALCLOSED (nth i lv (VNil))) ->
-  VALCLOSED v  ->
-  EXP (patternListScope lp) ⊢ ex
-  ->
-  FCLOSED (FCase2 v lp ex le lv)*)
-(*
-| FCLOSED_FCase2_g v lp ex le :
-  (forall i, i < length le -> EXP (patternListScope (nth i (map fst (map fst le)) nil)) ⊢ (nth i (map snd (map fst le)) (Val VNil))) ->
-  (forall i, i < length le -> EXP (patternListScope (nth i (map fst (map fst le)) nil)) ⊢ (nth i (map snd le) (Val VNil))) ->
-  VALCLOSED v  ->
-  EXP (patternListScope lp) ⊢ ex
-  ->
-  FCLOSED (FCase2_g v lp ex le) *)
-
-| FCLOSED_FLet l ex :
-  EXP l ⊢ ex
-  ->
-  FCLOSED (FLet l ex)
-
-
-| FCLOSED_FSeq ex :
-  EXPCLOSED ex
-  ->
-  FCLOSED (FSeq ex)
-
-| FCLOSED_FTry vl1 e2 vl2 e3 :
-  EXP vl1 ⊢ e2 ->
-  EXP vl2 ⊢ e3
-  ->
-  FCLOSED (FTry vl1 e2 vl2 e3)
-.
-
 Definition FSCLOSED (fs : FrameStack) := Forall FCLOSED fs.
-(* TODO: Should I use this definition, and what should be the default element? *)
-(* Definition FSCLOSED (fs : FrameStack) := (forall i, (i < length fs) -> FCLOSED (nth i fs (FValues [] []))). *)
 
-Lemma scoped_list_subscoped :
-  forall vals Γ ξ Γ', Forall (fun v => VAL Γ ⊢ v) vals -> SUBSCOPE Γ' ⊢ ξ ∷ Γ ->
-  SUBSCOPE length vals + Γ' ⊢ list_subst vals ξ ∷ Γ.
-Proof.
-  induction vals; intros; simpl; auto.
-  simpl. inversion H. intro. intros. destruct v.
-  * simpl. apply H3.
-  * simpl. specialize (IHvals _ _ _ H4 H0 v). apply IHvals. lia.
-Qed.
-
-Lemma scoped_list_idsubst :
-  forall vals Γ, Forall (fun v => VAL Γ ⊢ v) vals ->
-  SUBSCOPE length vals ⊢ list_subst vals idsubst ∷ Γ.
-Proof.
-  induction vals; intros. simpl.
-  unfold idsubst. intro. intros. inversion H0.
-  simpl. inversion H. intro. intros. destruct v.
-  * simpl. apply H2.
-  * simpl. apply IHvals; auto. lia.
-Qed.
-
-Lemma substcomp_scoped :
-  forall ξ σ Γ Δ Ω, SUBSCOPE Γ ⊢ ξ ∷ Δ -> SUBSCOPE Δ ⊢ σ ∷ Ω
-->
-  SUBSCOPE Γ ⊢ ξ >> σ ∷ Ω.
-Proof.
-  intros. intro. intros. unfold subscoped in H.
-  unfold ">>".
-  specialize (H v H1).
-  destruct (ξ v) eqn:D1.
-  * apply -> subst_preserves_scope_val; eassumption.
-  * specialize (H0 n H). auto.
-Qed.
-
-(* Needs help *)
-(*
-Theorem match_pattern_scoped : forall p v l Γ,
-  VAL Γ ⊢ v -> match_pattern p v = Some l
-->
-  Forall (fun v => VAL Γ ⊢ v) l.
-Proof.
-  induction p; intros.
-  * simpl in *. destruct v; inversion H0. break_match_hyp; inversion H0. auto.
-  * simpl in *. destruct v; inversion H0; subst; auto.
-  * simpl in *. destruct v; inversion H0. subst. auto.
-  * simpl. simpl in H0. destruct v; try congruence.
-    break_match_hyp; try congruence. break_match_hyp; try congruence. inversion H0.
-    subst. apply Forall_app. split.
-    - inversion H. subst. eapply IHp1. exact H3. auto.
-    - inversion H. subst. eapply IHp2. exact H4. auto.
-Qed.
-*)
-
-(* Not needed *)
-(*
-Ltac inversion_is_value :=
-match goal with
-| [ H: VAL _ ⊢ (ELet _ _ _) |- _ ] => inversion H
-| [ H: VAL _ ⊢ (ELetRec _ _ _ _) |- _ ] => inversion H
-| [ H: VAL _ ⊢ (EPlus _ _) |- _ ] => inversion H
-| [ H: VAL _ ⊢ (ECase _ _ _ _) |- _ ] => inversion H
-| [ H: VAL _ ⊢ (EApp _ _) |- _ ] => inversion H
-| [ H: VAL _ ⊢ (EVar _) |- _ ] => inversion H
-| [ H: VAL _ ⊢ (EFunId _) |- _ ] => inversion H
-| [ H: VAL _ ⊢ (ECons _ _) |- _ ] => inversion H
-end.
-*)
