src/Matching.v
@@ -1,0 +1,147 @@
+From CoreErlang Require Import ScopingLemmas Equalities Basics.
+Import ListNotations.
+
+Fixpoint match_pattern (p : Pat) (e : Val) : option (list Val) :=
+match p with
+| PVar => Some [e]
+(* | PPid x => match e with
+            | EPid p => if Nat.eqb p x then Some [] else None
+            | _      => None
+            end *)
+| PNil => match e with
+          | VNil => Some []
+          | _    => None
+          end
+| PLit l0 => match e with
+              | VLit l => if Lit_beq l l0 then Some [] else None
+              | _      => None
+              end
+| PCons p1 p2 => 
+  match e with
+  | VCons v1 v2 =>
+    match match_pattern p1 v1, match_pattern p2 v2 with
+    | Some l1, Some l2 => Some (l1 ++ l2)
+    | _      , _       => None
+    end
+  | _           => None
+  end
+| PTuple pl => match e with
+              | VTuple vl =>
+                        (fix match_and_bind_elements pl vl :=
+                        match pl with
+                        | [] => 
+                            match vl with
+                            | [] => Some []
+                            | _ => None
+                            end
+                        | p::ps => 
+                            match vl with
+                            | v::vs => 
+                                match (match_pattern p v) with
+                                | Some vl1 => 
+                                    match (match_and_bind_elements ps vs) with
+                                    | Some vl2 => Some (vl1 ++ vl2)
+                                    | _        => None
+                                    end
+                                | _ => None
+                                end
+                            | _ => None
+                            end 
+                        end) pl vl
+              | _ => None
+              end
+| PMap pl => match e with
+              | VMap vl => (fix match_and_bind_elements pl vl :=
+                          match pl with
+                          | [] => 
+                              match vl with
+                              | []  => Some []
+                              | _   => None
+                              end
+                          | (p1,p2)::ps => 
+                              match vl with
+                              | (v1,v2)::vs =>
+                                  match (match_pattern p1 v1), (match_pattern p2 v2) with
+                                  | Some vl1, Some vl1' =>
+                                      match (match_and_bind_elements ps vs) with
+                                      | Some vl2  => Some (vl1 ++ vl1' ++ vl2)
+                                      | _         => None
+                                      end
+                                  | _, _ => None
+                                  end
+                              | _ => None
+                              end
+                          end) pl vl
+              | _  => None
+              end
+end.
+
+Fixpoint match_pattern_list (pl : list Pat) (vl : list Val) : option (list Val) :=
+match pl,vl with
+  | (p::ps), (v::vs) => match match_pattern p v with
+                        | Some vs' => match match_pattern_list ps vs with
+                                      | Some vs'' => Some (vs'++vs'')
+                                      | None      => None
+                                      end
+                        | None => None
+                        end
+  | [], [] => Some []
+  | _, _ => None
+end.
+
+
+Theorem match_pattern_scoped : forall p v l Γ,
+  VAL Γ ⊢ v -> match_pattern p v = Some l
+->
+  Forall (fun v => VAL Γ ⊢ v) l.
+Proof.
+  induction p using Pat_ind2 with
+  (Q := Forall (fun p => forall v l Γ, 
+                  VAL Γ ⊢ v -> match_pattern p v = Some l
+                  -> Forall (fun v => VAL Γ ⊢ v) l))
+  (R := Forall (fun '(p1, p2) => (forall v l Γ, 
+  VAL Γ ⊢ v -> match_pattern p1 v = Some l
+  -> Forall (fun v => VAL Γ ⊢ v) l) /\
+  (forall v l Γ, 
+  VAL Γ ⊢ v -> match_pattern p2 v = Some l
+  -> Forall (fun v => VAL Γ ⊢ v) l))); try intros v l' Γ HΓ Hmatch; simpl in *; try now constructor.
+  * destruct v; try congruence. now inversion Hmatch.
+  * destruct v; try congruence.
+    destruct Lit_beq in Hmatch; inversion Hmatch. auto.
+  * inversion Hmatch. now constructor.
+  * destruct v; try congruence.
+    break_match_hyp; try congruence. break_match_hyp; try congruence. inversion Hmatch. inversion HΓ. subst. apply Forall_app. split.
+    - eapply IHp1. exact H3. auto.
+    - eapply IHp2. exact H4. auto.
+  * destruct v; try congruence. inversion HΓ; subst. clear HΓ.
+    apply indexed_to_forall in H1.
+    generalize dependent l'; generalize dependent l; induction l0;
+    intros l H l' Hmatch.
+    - destruct l. 2: congruence. now inversion Hmatch.
+    - inversion H1; subst; clear H1.
+      destruct l. congruence.
+      do 2 (break_match_hyp; try congruence).
+      inversion H; subst; clear H.
+      specialize (IHl0 H4 l H5 _ Heqo0). inversion Hmatch; subst. clear Hmatch.
+      apply Forall_app; split; auto.
+      clear IHl0 Heqo0. eapply H2 in Heqo; eauto.
+  * destruct v; try congruence. inversion HΓ; subst. clear HΓ.
+    generalize dependent l'; generalize dependent l; induction l0;
+    intros l H l' Hmatch.
+    - destruct l. 2: { destruct p; congruence. } now inversion Hmatch.
+    - destruct l. congruence.
+      do 5 (break_match_hyp; try congruence).
+      inversion H; subst; clear H.
+      inversion Hmatch; subst. clear Hmatch.
+      destruct H4.
+      apply Forall_app; split;[|apply Forall_app; split].
+      3: {
+        eapply IHl0.
+        - intros. apply (H0 (S i)). simpl. lia.
+        - intros. apply (H2 (S i)). simpl. lia.
+        - apply H5.
+        - assumption.
+      }
+      + eapply H. 2: eassumption. apply (H0 0). simpl. lia.
+      + eapply H1. 2: eassumption. apply (H2 0). simpl. lia.
+Qed.
